Semantics/I_Semantics.thy
@@ -22,103 +22,13 @@ eed
 
 *)
 
-consts Length :: "'a \<Rightarrow> nat"
-
-overloading
-  Length0 \<equiv> "Length :: unit \<Rightarrow> nat"
-begin
-
-fun Length0 :: "unit \<Rightarrow> nat" where
-  "Length0 () = 0"
-
-end
-
-value [nbe] "Length () :: nat"
-
-
-
-(*consts LInst :: "'full itself \<Rightarrow> 'i \<Rightarrow> 'xp \<Rightarrow> ('i, 'xp, 'a) mpack"*)
-(*
-consts LInst :: "('w, 'x, 'y) mpack itself \<Rightarrow> 'i \<Rightarrow> 'xp \<Rightarrow> ('w, 'x, 'y) mpack"
-
-overloading
-  LInst0 \<equiv> "LInst :: ('i, 'xp, 'a) mpack itself \<Rightarrow> 'i \<Rightarrow> 'xp \<Rightarrow> ('i, 'xp, 'a) mpack"
-begin
-
-fun LInst0 :: "('i, 'xp, 'a) mpack itself \<Rightarrow> 'i \<Rightarrow> 'xp \<Rightarrow> ('i, 'xp, 'a) mpack" where
-  "LInst0 tf i xp = (Inl i, xp) "
-end 
-
-
-
-lemmas [code] = LInst0.simps
-
-
-value "LInst () () :: (unit, unit, unit) syn_i"
-
-*)
-
-(*
-declare [[coercion_enabled]]
-
-fun natid :: "nat \<Rightarrow> nat" where
-"natid x = x"
-
-fun swap :: "('a \<Rightarrow> 'b) \<Rightarrow> ('b \<Rightarrow> 'a) \<Rightarrow> ('a + 'b) \<Rightarrow> ('b + 'a)"
-  where
-"swap f g (Inl x) = Inr x"
-| "swap f g (Inr x) = Inl x"
-
-declare [[coercion_map swap]]
-*)
-
-value \<open>STR''abc'' :: string\<close>
-
-
-consts GetLen :: "'a \<Rightarrow> nat"
-overloading
-  GetLen0 \<equiv> "GetLen :: unit \<Rightarrow> nat"
-begin
-
-fun GetLen0 :: "unit \<Rightarrow> nat" where
-  "GetLen0 () = 0"
-
-end
-
-declare GetLen0.simps [simp]
-
-value [nbe] "GetLen () :: nat"
-
-consts GetNat :: "'a \<Rightarrow> nat"
-overloading
-  Get0 \<equiv> "GetNat :: nat \<Rightarrow> nat"
-begin
-
-fun Get0 :: "nat \<Rightarrow> nat" where
-  "Get0 n = n"
-
-end
-
-lemma testt : "GetNat (1 :: nat) = 1"
-  apply(simp)
-  done
-
-value [nbe] "case (GetNat (0 :: nat) :: nat) of 0 \<Rightarrow> False | _ \<Rightarrow> True"
-
-(*
-
-value "(\<lambda> (x, y) . x) (2 :: nat, undefined :: nat)"
-
-value "fst ((3, undefined) :: nat * nat)"
-*)
-locale I_Semantics_Sig =
+locale I_Semantics_Sig = Syn_I +
   fixes xr :: "'rs itself"
-  fixes ms :: "'mstate itself"
-  fixes i_sem :: "'i \<Rightarrow> 'mstate => 'mstate \<Rightarrow> bool"
-
+  fixes i_sem :: "'a \<Rightarrow> 'mstate => 'mstate \<Rightarrow> bool"
 
 locale I_Semantics = I_Semantics_Sig 
 begin
+print_context
 
 (* 2 approaches.
    approach 1: i_semantics builds a gensym semantics "from nothing"
@@ -150,12 +60,12 @@ do we need another extension point to allow for this?. *)
 
 print_context
 
-inductive x_sem_i :: "  ('c, 'xp, 'xs) syn_i \<Rightarrow> 
-                         'b \<Rightarrow>
-                         'b \<Rightarrow>
-                          childpath \<Rightarrow> ('c, 'xp, 'xs) syn_i gensyn \<Rightarrow> 
-                          ('a) gs_result \<Rightarrow> bool" where
-"i_sem i m m' \<Longrightarrow> x_sem_i (LInst i xp) m m' cp t GRUnhandled"
+inductive x_sem_i :: "  ('a, 'b, 'c) mpackf \<Rightarrow> 
+                         'e \<Rightarrow>
+                         'e \<Rightarrow>
+                          childpath \<Rightarrow> ('a, 'b, 'c) mpackf gensyn \<Rightarrow> 
+                          ('d) gs_result \<Rightarrow> bool" where
+"i_sem i m m' \<Longrightarrow> x_sem_i (LInst xp i) m m' cp t GRUnhandled"
 
 (* We still need a way to handle different kinds of gs results *)
 
@@ -165,8 +75,6 @@ as this would require a recursive semantics; we use nosem *)
 
 end
 
-
-locale Gensyn_Semantics_I = I_Semantics 
 
 (* this seems like a bad idea unless we can make things work out
    when we combine together multiple locales *)
@@ -181,11 +89,7 @@ sublocale Gensyn_Semantics_I \<subseteq> Gensyn_Semantics_Base_Sig
 (* i think the problem with this is that we cannot further
 sub-locale-ize I_Semantics *)
 
-(* test - small programming language for arithmetic *)
-datatype calc =
-  AccAdd nat
-  | AccSub nat
-  | AccReset
+
 
 fun calc_sem :: "calc \<Rightarrow> nat \<Rightarrow> nat" where
 "calc_sem (AccAdd x) n = x + n"
@@ -195,15 +99,20 @@ fun calc_sem :: "calc \<Rightarrow> nat \<Rightarrow> nat" where
 inductive calc_semb :: "calc \<Rightarrow> nat \<Rightarrow> nat \<Rightarrow> bool" where
 "\<And> c n n' . calc_sem c n = n' \<Longrightarrow> calc_semb c n n'"
 
+print_locale I_Semantics
+
+(*
 interpretation I_Semantics_Calc :
-  I_Semantics "TYPE(unit)" _ calc_semb
+  I_Semantics
+  reify denote reify denote
+      bail "TYPE(unit)" calc_semb
   done
 
 
 interpretation Gensyn_Semantics_Calc :
   Gensyn_Semantics "TYPE(unit)" _ I_Semantics_Calc.x_sem_i
   done
-
+*)
 
 locale Gensyn_Base_Oneshot =
   fixes ms :: "'mstate itself"
@@ -228,8 +137,12 @@ inductive x_sem_oneshot :: "'x \<Rightarrow>
 
 end
 
+print_locale! I_Semantics
+
+
 locale I_Semantics_Oneshot = I_Semantics
 
+print_locale! I_Semantics_Oneshot
 
 sublocale I_Semantics_Oneshot \<subseteq> Gensyn_Base_Oneshot
   where x_sem = x_sem_i
@@ -240,15 +153,21 @@ sublocale I_Semantics_Oneshot \<subseteq> Gensyn_Semantics
   where x_sem = x_sem_oneshot
   done
 
-interpretation Gensyn_Semantics_Calc_Oneshot :
-  I_Semantics_Oneshot "TYPE(unit)" _ calc_semb
+print_locale! I_Semantics_Oneshot
+
+
+global_interpretation Gensyn_Semantics_Calc_Oneshot? :
+  I_Semantics_Oneshot reify denote reify denote bail "TYPE(unit)" calc_semb
   done
 
-term Gensyn_Semantics_Calc.gensyn_sem
+term "Gensyn_Semantics_Calc_Oneshot.LInst"
 
-lemma testout1 : "Gensyn_Semantics_Calc_Oneshot.gensyn_sem (G (LInst AccReset ()) []) [] 0 42"
-  apply(rule Gensyn_Semantics_Calc_Oneshot.gensyn_sem.intros) apply(auto)
-  apply(rule Gensyn_Base_Oneshot.x_sem_oneshot.intros)
+term gensyn_sem
+
+lemma testout1 : "gensyn_sem 
+    (G (LInst () AccReset) []) [] 0 42"
+  apply(rule gensyn_sem.intros) apply(auto)
+  apply(rule x_sem_oneshot.intros)
   apply(rule I_Semantics.x_sem_i.intros)
   apply(rule calc_semb.intros)
   apply(auto)
